Work on VCG with Daniel

compiler/dafny/vcg/dafny_wp_calcScript.sml
@@ -21,20 +21,33 @@ Datatype:
               ; reads     : exp list
               ; decreases : exp list
               ; outs      : (mlstring # type) list
-              ; mods      : exp list |>
+              ; mods      : exp list
+              ; rank      : num |>
 End
 
 Datatype:
   met = Method mlstring met_spec statement
 End
 
+Overload True = “Lit (BoolL T)”;
 Overload False = “Lit (BoolL F)”;
 
-Definition eval_true_def[simp]:
-  eval_true st env e ⇔
+Definition eval_exp_def:
+  eval_exp st env e v ⇔
     ∃ck1 ck2.
       evaluate_exp (st with clock := ck1) env e =
-        (st with clock := ck2, Rval (BoolV T))
+        (st with clock := ck2, Rval v)
+End
+
+Definition eval_stmt_def:
+  eval_stmt st env body st' ret =
+    ∃ck1 ck2.
+      evaluate_stmt (st with clock := ck1) env body =
+        (st' with clock := ck2, ret)
+End
+
+Definition eval_true_def:
+  eval_true st env e ⇔ eval_exp st env e (BoolV T)
 End
 
 Definition valid_def:
@@ -50,53 +63,108 @@ Definition conj_def:
 End
 
 Overload "imp" = “BinOp Imp”
+Overload "int_lt" = “BinOp Lt”
+Overload "dfy_eq" = “BinOp Eq”
 
 Overload "not" = “UnOp Not”
+
+Definition CanEval_def: (* beautiful or not.. *)
+  CanEval e = dfy_eq e e
+End
+
+Theorem eval_true_CanEval:
+  eval_true st env (CanEval e) ⇒ ∃v. eval_exp st env e v
+Proof
+  gvs [eval_true_def,CanEval_def,evaluate_exp_def,eval_exp_def]
+  \\ gvs [AllCaseEqs(),PULL_EXISTS,do_sc_def,do_bop_def]
+  \\ cheat
+QED
+
+Theorem EVERY_eval_true_CanEval:
+  EVERY (eval_true st env) (MAP CanEval args) ⇒
+  ∃in_vs. LIST_REL (eval_exp st env) args in_vs
+Proof
+  Induct_on ‘args’ \\ gvs [] \\ rw []
+  \\ res_tac \\ drule eval_true_CanEval \\ strip_tac
+  \\ rpt $ pop_assum $ irule_at Any
+QED
+
+Definition decrease_lt_def:
+  decrease_lt [] [] = False ∧
+  decrease_lt [] ys = True ∧
+  decrease_lt xs [] = False ∧
+  decrease_lt (x::xs) (y::ys) =
+    if LENGTH xs = LENGTH ys then
+      If (dfy_eq x y) (decrease_lt xs ys) (int_lt x y)
+    else if LENGTH xs < LENGTH ys then True else False
+End
+
+Definition decreases_check_def:
+  decreases_check (now_r,now) (old_r:num,old) =
+    if now_r ≠ old_r then
+      if now_r < old_r then [] else [False]
+    else [decrease_lt now old]
+End
+
+Definition wrap_old_def:
+  wrap_old (x,es) = (x,MAP Old es)
+End
 
 Inductive stmt_wp:
 [~Skip:]
   ∀m ens post.
-    stmt_wp m post Skip (post:exp list) (ens:exp list)
+    stmt_wp m post Skip (post:exp list) (ens:exp list) decs
 [~Assert:]
   ∀m ens post e.
-    stmt_wp m (e::post) (Assert e) (post:exp list) (ens:exp list)
+    stmt_wp m (e::post) (Assert e) (post:exp list) (ens:exp list) decs
 [~Return:]
   ∀m ens post.
-    stmt_wp m (ens:exp list) Return (post:exp list) (ens:exp list)
+    stmt_wp m (ens:exp list) Return (post:exp list) (ens:exp list) decs
 [~Then:]
   ∀m s1 s2 pre1 pre2 post ens.
-    stmt_wp m pre1 s1 pre2 ens ∧
-    stmt_wp m pre2 s2 post ens
+    stmt_wp m pre1 s1 pre2 ens decs ∧
+    stmt_wp m pre2 s2 post ens decs
     ⇒
-    stmt_wp m pre1 (Then s1 s2) post ens
+    stmt_wp m pre1 (Then s1 s2) post ens decs
 [~If:]
   ∀m s1 s2 pre1 pre2 post ens g.
-    stmt_wp m pre1 s1 post ens ∧
-    stmt_wp m pre2 s2 post ens
+    stmt_wp m pre1 s1 post ens decs ∧
+    stmt_wp m pre2 s2 post ens decs
     ⇒
-    stmt_wp m [imp g (conj pre1); imp (not g) (conj pre2)] (If g s1 s2) post ens
+    stmt_wp m [imp g (conj pre1); imp (not g) (conj pre2)] (If g s1 s2) post ens decs
 [~Assign:]
   ∀m ret_names exps l post ens.
     LIST_REL (λr (n,ty). r = VarLhs n) (MAP FST l) ret_names ∧
     LIST_REL (λr e. r = ExpRhs e) (MAP SND l) exps
     ⇒
-    stmt_wp m [Let (ZIP (ret_names,exps)) (conj post)] (Assign l) post ens
+    stmt_wp m [Let (ZIP (ret_names,exps)) (conj post)] (Assign l) post ens decs
 [~MetCall:]
   ∀m mname mspec mbody args ret_names rets post ens.
     Method mname mspec mbody ∈ m ∧
     LENGTH mspec.ins = LENGTH args ∧
+    ALL_DISTINCT (MAP FST mspec.ins ++ MAP FST mspec.outs) ∧
     LIST_REL (λr rn. r = VarLhs (FST rn)) rets ret_names ∧
-    ⊢ (imp (conj mspec.ens) (Let (ZIP (ret_names,MAP (λ(m,ty). Var m) mspec.outs)) (conj post)))
+    ⊢ (imp (conj mspec.ens)
+         (Let (ZIP (ret_names,MAP (λ(m,ty). Var m) mspec.outs)) (conj post)))
     ⇒
-    stmt_wp m [Let (ZIP (mspec.ins,args)) (conj mspec.reqs)]
-              (MetCall rets mname args) post ens
+    stmt_wp m (Let (ZIP (mspec.ins,args)) (conj mspec.reqs) ::
+               MAP CanEval args ++
+               decreases_check (mspec.rank,
+                                MAP (Let (ZIP (mspec.ins,args))) mspec.decreases)
+                               (wrap_old decs))
+              (MetCall rets mname args) post ens decs
 End
 
-Inductive adjust_calls:
-  T ⇒
-  adjust_calls decreases mutrec body
+Definition proved_methods_def:
+  proved_methods m ⇔
+    ∀name mspec body.
+      Method name mspec body ∈ m ⇒
+      ∃wp_pre.
+        stmt_wp m wp_pre body [False] mspec.ens (mspec.rank, mspec.decreases) ∧
+        ⊢ (imp (conj mspec.reqs) (conj wp_pre))
 End
 
+(*
 Inductive proved_methods:
 [~empty:]
   proved_methods {}
@@ -119,20 +187,20 @@ Inductive proved_methods:
     ⇒
     proved_methods (mutrec ∪ m)
 End
-
-Definition eval_stmt_def:
-  eval_stmt st env body st' ret =
-    ∃ck1 ck2.
-      evaluate_stmt (st with clock := ck1) env body =
-        (st' with clock := ck2, ret)
-End
+*)
 
 Definition conditions_hold_def:
   conditions_hold st env ⇔ EVERY (eval_true st env)
 End
 
 Definition compatible_env_def:
-  compatible_env env m = ¬env.is_running
+  compatible_env env m ⇔
+    ¬env.is_running ∧
+    (∀name mspec body.
+       Method name mspec body ∈ m ⇒
+       get_member name env.prog =
+       SOME (Method name mspec.ins mspec.reqs mspec.ens
+                    mspec.reads mspec.decreases mspec.outs mspec.mods body))
 End
 
 Theorem imp_conditions_hold:
@@ -154,6 +222,156 @@ Definition methods_sound_def:
                  conditions_hold st' env mspec.ens
 End
 
+Triviality WF_lemma:
+  WF (prim_rec$< LEX SHORTLEX prim_rec$<)
+Proof
+  irule pairTheory.WF_LEX
+  \\ irule_at Any listTheory.WF_SHORTLEX
+  \\ rewrite_tac [prim_recTheory.WF_LESS]
+QED
+
+Triviality WF_ind =
+  MATCH_MP relationTheory.WF_INDUCTION_THM WF_lemma;
+
+Definition evaluate_exp_total_def:
+  evaluate_exp_total st env e =
+    some v. eval_exp st env e v
+End
+
+Definition eval_decreases_def:
+  eval_decreases st env [] = SOME [] ∧
+  eval_decreases st env (e::es) =
+    case evaluate_exp_total st env e, eval_decreases st env es of
+    | (SOME (IntV i), SOME rest) =>
+        if i < 0 then NONE else SOME (Num i :: rest)
+    | _ => NONE
+End
+
+Definition eval_measure_def:
+  eval_measure st env (rank:num,es) =
+    (rank, THE (eval_decreases st env es))
+End
+
+Theorem False_thm[simp,local]:
+  conditions_hold st env [False] = F
+Proof
+  simp [conditions_hold_def,eval_true_def,evaluate_exp_def,eval_exp_def]
+QED
+
+Theorem evaluate_stmt_MetCall:
+  get_member mname env.prog =
+    SOME (Method name ins reqs ens rds decrs outs mods body) ∧
+  LIST_REL (eval_exp st env) args in_vs ∧
+  set_up_call st (MAP FST ins) in_vs (MAP FST outs) = SOME st1 ∧
+  eval_stmt st1 env body st2 (Rstop Sret) ∧
+  OPT_MMAP (read_local st2.locals) out_ns = SOME out_vs ∧
+  LENGTH rets = LENGTH out_vs ∧
+  assign_values (restore_caller st2 st0) env rets out_vs = (st',Rcont)
+  ⇒
+  eval_stmt st env (MetCall rets mname args) st' Rcont
+Proof
+  cheat
+QED
+
+Theorem stmt_wp_sound:
+  ∀m reqs stmt post ens decs.
+    stmt_wp m reqs stmt post ens decs ⇒
+    ∀st env.
+      (∀st' name' mspec' body'.
+          ($< LEX SHORTLEX $<)
+            (eval_measure st' env (mspec'.rank,mspec'.decreases))
+            (eval_measure st env (wrap_old decs)) ∧
+          Method name' mspec' body' ∈ m ∧ st'.locals_old = st'.locals ∧
+          st'.heap_old = st'.heap ∧ conditions_hold st' env mspec'.reqs ∧
+          compatible_env env m ⇒
+          ∃st''.
+            eval_stmt st' env body' st'' (Rstop Sret) ∧
+            conditions_hold st'' env mspec'.ens) ∧
+      conditions_hold st env reqs ∧ compatible_env env m ⇒
+      ∃st' ret.
+        eval_stmt st env stmt st' ret ∧
+        case ret of
+        | Rstop Sret => conditions_hold st' env ens
+        | Rcont => conditions_hold st' env post
+        | _ => F
+Proof
+
+  Induct_on ‘stmt_wp’ \\ rpt strip_tac
+  >~ [‘MetCall rets mname args’] >-
+   (irule_at Any evaluate_stmt_MetCall \\ gvs []
+    \\ qpat_assum ‘compatible_env env m’ mp_tac
+    \\ rewrite_tac [compatible_env_def]
+    \\ strip_tac
+    \\ pop_assum drule
+    \\ strip_tac \\ gvs []
+    \\ gvs [conditions_hold_def]
+    \\ drule EVERY_eval_true_CanEval \\ strip_tac
+    \\ first_assum $ irule_at Any
+    \\ gvs [set_up_call_def]
+    \\ simp [safe_zip_def]
+    \\ imp_res_tac LIST_REL_LENGTH \\ gvs []
+    \\ qpat_abbrev_tac ‘new_l = REVERSE _’
+    \\ qmatch_goalsub_abbrev_tac ‘eval_stmt st1’
+    \\ first_x_assum $ drule_at $ Pos $ el 2
+    \\ disch_then $ qspec_then ‘st1’ mp_tac
+    \\ impl_tac
+    >-
+     (reverse $ rpt conj_tac
+      >- cheat
+      >- gvs [Abbr‘st1’]
+      >- gvs [Abbr‘st1’]
+      \\ PairCases_on ‘decs’ \\ gvs [wrap_old_def]
+      \\ qpat_x_assum ‘EVERY _ (decreases_check _ _)’ mp_tac
+      \\ simp [decreases_check_def] \\ cheat)
+    \\ cheat)
+
+  \\ cheat
+QED
+
+Theorem eval_measure_wrap_old:
+  st.locals_old = st.locals ∧ st.heap_old = st.heap ⇒
+  eval_measure st env (wrap_old decs) =
+  eval_measure st env decs
+Proof
+  cheat
+QED
+
+Theorem methods_lemma[local]:
+  ∀m.
+    proved_methods m ⇒
+    ∀x st name mspec body env.
+      x = eval_measure st env (mspec.rank, mspec.decreases) ∧
+      Method name mspec body ∈ m ∧
+      st.locals_old = st.locals ∧
+      st.heap_old = st.heap ∧
+      conditions_hold st env mspec.reqs ∧ compatible_env env m ⇒
+      ∃st'. eval_stmt st env body st' (Rstop Sret) ∧
+            conditions_hold st' env mspec.ens
+Proof
+  gen_tac
+  \\ disch_tac
+  \\ ho_match_mp_tac WF_ind
+  \\ rpt strip_tac
+  \\ gvs [PULL_FORALL]
+  \\ last_x_assum (drule o SRULE [proved_methods_def])
+  \\ strip_tac
+  \\ drule stmt_wp_sound
+  \\ disch_then $ qspecl_then [‘st’,‘env’] mp_tac
+  \\ impl_tac >-
+   (asm_rewrite_tac []
+    \\ drule_all imp_conditions_hold \\ strip_tac \\ gvs []
+    \\ rpt strip_tac
+    \\ gvs [eval_measure_wrap_old]
+    \\ simp [SF SFY_ss])
+  \\ gvs [False_thm]
+  \\ strip_tac
+  \\ every_case_tac \\ gvs []
+  \\ rpt $ first_assum $ irule_at Any
+QED
+
+Theorem methods_correct = SRULE [] methods_lemma;
+
+(*
 Theorem stmt_wp_sound:
   ∀m reqs stmt post ens.
     stmt_wp m reqs stmt post ens ⇒
@@ -183,12 +401,6 @@ Proof
     \\ last_x_assum $ irule_at Any
     \\ gvs [dafny_semanticPrimitivesTheory.state_component_equality])
   \\ cheat
-QED
-
-Theorem False_thm:
-  conditions_hold st env [False] = F
-Proof
-  simp [conditions_hold_def,eval_true_def,evaluate_exp_def]
 QED
 
 Theorem proved_methods_sound:
@@ -233,3 +445,4 @@ Proof
   \\ gvs [False_thm]
   \\ cheat
 QED
+*)
